More refactoring

DerivationTests.v
@@ -1,24 +1,29 @@
 Require Import Derivation.
-Require Import GrammarSymbol.
-Require Import Grammar.
 Require Import ExampleGrammars.
+Require Import Grammar.
 Require Import List.
 Require Import ParseTree.
-Require Import Parser.
+Require Import ParserTactics.
 Require Import String.
 Import ListNotations.
 Open Scope string_scope.
 
-Definition input1 := ["if" ; "num" ; "==" ; "num" ; "then" ; "print" ; "num" ; "==" ; "num" ; "else" ; "print" ; "num" ; "==" ; "num"].
-Example derivation1 : (@derives g311) (NT "S") input1 (Node "S" [Leaf "if" ;
-                                                                 Node "E" [Leaf "num" ; Leaf "==" ; Leaf "num"] ;
-                                                                 Leaf "then" ;
-                                                                 Node "S" [Leaf "print" ;
-                                                                           Node "E" [Leaf "num" ; Leaf "==" ; Leaf "num"]] ;
-                                                                 Leaf "else" ;
-                                                                 Node "S" [Leaf "print" ;
-                                                                           Node "E" [Leaf "num" ; Leaf "==" ; Leaf "num"]]]).
+Definition input1 :=
+  ["if" ; "num" ; "==" ; "num" ; "then" ; "print" ; "num" ; "==" ; "num" ; "else" ; "print" ; "num" ; "==" ; "num"].
 
+Definition parseTree1 :=
+  (Node "S" [Leaf "if" ;
+             Node "E" [Leaf "num" ; Leaf "==" ; Leaf "num"] ;
+             Leaf "then" ;
+             Node "S" [Leaf "print" ;
+                       Node "E" [Leaf "num" ; Leaf "==" ; Leaf "num"]] ;
+             Leaf "else" ;
+             Node "S" [Leaf "print" ;
+                       Node "E" [Leaf "num" ; Leaf "==" ; Leaf "num"]]]).
+
+(* Manual proof of a derivation (don't do this again) *)
+Example derivesTest1 :
+  (@derives g311) (NT "S") input1 parseTree1.
 Proof.
   apply derivesNT with (prod := (NT "S", [T "if" ; NT "E" ; T "then" ; NT "S" ; T "else" ; NT "S"])); simpl; split.
   - left. reflexivity.
@@ -85,30 +90,9 @@ Proof.
     + reflexivity.
 Defined.
 
-Ltac crush := repeat match goal with
-                     | |- _ /\ _ => split
-                     | |- In _ _ => repeat (try (left ; reflexivity) ; right)
-                     | |- derives (T _) _ _ => apply derivesT
-                     | |- derives2 (T _) _  => apply derivesT2
-                     | |- derivesList (T ?s :: _) _ _ => let tName := s
-                                                         in  apply derivesCons with (prefix := [tName])
-                     | |- derivesList2 (T ?s :: _) _  => let tName := s
-                                                         in  apply derivesCons2 with (prefix := [tName])
-                     | |- derivesList [] _ _ => apply derivesNil
-                     | |- derivesList2 [] _  => apply derivesNil2
-                     | |- ?P = ?P => reflexivity
-                     | |- _ => simpl
-                     end.
-
 (* A more automated proof of the same derivation. *)
-Example derivation2 : (@derives g311) (NT "S") input1 (Node "S" [Leaf "if" ;
-                                                                 Node "E" [Leaf "num" ; Leaf "==" ; Leaf "num"] ;
-                                                                 Leaf "then" ;
-                                                                 Node "S" [Leaf "print" ;
-                                                                           Node "E" [Leaf "num" ; Leaf "==" ; Leaf "num"]] ;
-                                                                 Leaf "else" ;
-                                                                 Node "S" [Leaf "print" ;
-                                                                           Node "E" [Leaf "num" ; Leaf "==" ; Leaf "num"]]]).
+Example derivesTest2 :
+  (@derives g311) (NT "S") input1 parseTree1.
 Proof.
   apply derivesNT with (prod := (NT "S", [T "if" ; NT "E" ; T "then" ; NT "S" ; T "else" ; NT "S"])); crush.
   apply derivesCons with (prefix := ["num" ; "==" ; "num"]).
@@ -128,6 +112,8 @@ Proof.
       * crush.
 Defined.
 
+(* Proof using the binary derivation relation, which doesn't include the notion
+   of a parse tree or semantic value *)
 Example derives2Test : (@derives2 g311) (NT "S") input1.
 Proof.
   unfold input1.
