Derivation.v
@@ -1,32 +1,9 @@
-Require Import GrammarSymbol.
 Require Import Grammar.
 Require Import ParseTree.
 Require Import List.
 Require Import String.
 Require Import Parser.
 Import ListNotations.
-
-(* To do : rephrase this in terms of a grammar and it's productions.
-   At the moment, NT and subtrees in derivesNT could be from different productions. *)
-
-(* Binary version of the derives relation *)
-Inductive derives2 {g : grammar} : symbol -> list string -> Prop :=
-| derivesEPS2 : derives2 EPS []
-| derivesT2  : forall (tName : string),
-    derives2 (T tName)  [tName]
-| derivesNT2 : forall (ntName : string) (prod : production) (tokens : list string),
-    In prod g /\ derivesList2 (rhs prod) tokens /\ lhs prod = (NT ntName) ->
-    derives2 (NT ntName) tokens
-            
-with derivesList2 {g : grammar} : list symbol -> list string -> Prop :=
-     | derivesNil2  : derivesList2 nil nil
-     | derivesCons2 :
-         forall (hdRoot : symbol) (prefix : list string),
-           derives2 hdRoot prefix ->
-           
-           forall (tlRoots : list symbol) (suffix : list string),
-             derivesList2 tlRoots suffix ->
-             derivesList2 (hdRoot :: tlRoots) (prefix ++ suffix).
 
 Inductive derives {g : grammar} : symbol -> list string -> parse_tree -> Prop :=
 | derivesT  : forall (tName : string),
@@ -46,21 +23,22 @@ with derivesList {g : grammar} : list symbol -> list string -> list parse_tree -
              
              derivesList (hdRoot :: tlRoots) (prefix ++ suffix) (hdSubtree :: tlSubtrees).
 
-Definition g := [(NT "noun phrase", [T "the" ; T "tiger"])].
 
-(* This proof shouldn't succeed, because there's no grammar with the production 
-   NT "noun phrase" -> [T "the" ; T "tiger"] *)
-(* Edit -- now it does succeed, because I've added the notion of a grammar to the "derives" definition. *)
-Example foo : (@derives g) (NT "noun phrase") ["the" ; "tiger"] (Node "noun phrase" [Leaf "the" ; Leaf "tiger"]).
-Proof.
-  apply derivesNT with (prod := (NT "noun phrase", [T "the" ; T "tiger"])).
-  split.
-  - simpl. left. reflexivity.
-  - simpl. split.
-    + apply derivesCons with (prefix := ["the"]).
-      { apply derivesT. }
-      { apply derivesCons with (prefix := ["tiger"]).
-        apply derivesT.
-        apply derivesNil. }
-    + reflexivity.
-Defined.
+(* Binary version of the derives relation *)
+Inductive derives2 {g : grammar} : symbol -> list string -> Prop :=
+| derivesEPS2 : derives2 EPS []
+| derivesT2  : forall (tName : string),
+    derives2 (T tName)  [tName]
+| derivesNT2 : forall (ntName : string) (prod : production) (tokens : list string),
+    In prod g /\ derivesList2 (rhs prod) tokens /\ lhs prod = (NT ntName) ->
+    derives2 (NT ntName) tokens
+            
+with derivesList2 {g : grammar} : list symbol -> list string -> Prop :=
+     | derivesNil2  : derivesList2 nil nil
+     | derivesCons2 :
+         forall (hdRoot : symbol) (prefix : list string),
+           derives2 hdRoot prefix ->
+           
+           forall (tlRoots : list symbol) (suffix : list string),
+             derivesList2 tlRoots suffix ->
+             derivesList2 (hdRoot :: tlRoots) (prefix ++ suffix).
