ExampleGrammars.v
@@ -2,6 +2,7 @@ Require Import Grammar.
 Require Import List.
 Import ListNotations.
 
+(* Grammar 3.11 from Appel's "Modern Compiler Implementation in ML" *)
 Definition g311 : grammar :=
   [
     (NT "S", [T "if"; NT "E"; T "then"; NT "S"; T "else"; NT "S"]);
@@ -12,3 +13,12 @@ Definition g311 : grammar :=
    (NT "L", [T ";"; NT "S"; NT "L"]);
    
    (NT "E", [T "num"; T "=="; T "num"])].
+
+(* Grammar 3.12 from Appel's "Modern Compiler Implementation in ML" *)
+Definition g312 : grammar :=
+  [(NT "Z", [T "d"]); 
+   (NT "Z", [NT "X"; NT "Y"; NT "Z"]);
+   (NT "Y", [EPS]);
+   (NT "Y", [T "c"]);
+   (NT "X", [NT "Y"]);
+   (NT "X", [T "a"])].
